MLIR/Examples/EndToEndLinalg.lean
@@ -14,9 +14,9 @@ def matmul_ein := [ein_factor| x_k_i x^i_l]
 
 -- | Mix into MLIR definitions.
 def matmul_linalg := [mlir_op|
-   func @"main"(%a: tensor<?×?:f32>, %b: tensor<?×?:f32>, %out: tensor<?×?:f32>) -> () {
-     ^entry():
-      a^i b_i (%out)
+   func @"main"(%a: tensor<?×?:f32>, %b: tensor<?×?:f32>, %out: tensor<?×?:f32>)  {
+      ^entry:
+        a^i b_i (%out)
     }
 ]
 
