MLIR/LLVM.lean
@@ -1,0 +1,5 @@
+import MLIR.AST
+import MLIR.EDSL
+
+-- Definition of LLVM as an MLIR dialect.
+-- https://mlir.llvm.org/docs/TargetLLVMIR/#conversion-to-the-llvm-dialect
